src/Language/PlutusIR/Transform/LetNonRec/Static.v
@@ -4,151 +4,19 @@ Require Import Coq.Program.Basics.
 Require Import Coq.Lists.List.
 Import ListNotations.
 
-Local Open Scope context_scope.
+Require Import PlutusCert.Language.PlutusIR.Semantics.Static.
+Require Import PlutusCert.Language.PlutusIR.Semantics.Static.Implementations.Named.
+Import NamedTerm.
 
-(*
-Theorem CNR_Binding__preserves_wellformedness : forall b f_b bs,
-    ctx |-ok (TermBind Strict (VarDecl v ty) t_bound) ->
-    CNR_Binding b f_b ->
-    appendContext (binds bs) ctx |-+ (f_b t_bound) : T.
+Definition P ctx t1 T := forall t2, CNR_Term t1 t2 -> ctx |-+ t2 : T.
 
-
-with CNR_Binding : Binding -> (Term -> Term) -> Type :=
-  | CNR_Desugar : forall {v t_bound t_bound' ty},
-      CNR_Term t_bound t_bound' ->
-      CNR_Binding
-        (TermBind Strict (VarDecl v ty) t_bound)
-        (fun t_bs => Apply (LamAbs v ty t_bs) t_bound')
-  .
-
-Theorem CNR_Bindings__preserves_typing : forall bs ctx t_body T t_body' f_bs,
-    (forall b : Binding, In b bs -> binding_well_formed ctx b) ->
-    appendContexts (fold_right appendContexts Nil (map binds bs)) ctx |-+ t_body : T ->
-    CNR_Term t_body t_body' ->
-    (forall t2 : Term, CNR_Term t_body t2 -> appendContexts (fold_right appendContexts Nil (map binds bs)) ctx |-+ t2 : T) ->
-    CNR_Bindings bs f_bs ->
-    ctx |-+ (fold_right apply t_body' f_bs) : T.
-Proof.
-  intros.
-  generalize dependent ctx.
-  generalize dependent t_body.
-  generalize dependent T.
-  generalize dependent t_body'.
-  induction X0.
-  - intros.
-    simpl.
-    apply H1.
-    apply X.
-  - intros.
-    simpl.
-    simpl in H1.
-    inversion c. subst.
-    *)
-
-    
-
-Theorem CNR_Term__preserves_typing : forall t1 t2 T ctx,
+Theorem CNR_Term__preserves_typing : forall ctx t1 T,
     ctx |-+ t1 : T ->
-    CNR_Term t1 t2 ->
-    ctx |-+ t2 : T.
+    P ctx t1 T.
 Proof.
-  intros t1 t2 T ctx Ht1.
-  generalize dependent t2.
-  induction Ht1. 
-  - intros t2 H_CNR.
-    inversion H_CNR.
-    + subst.
+  eapply has_type_rec.
+  - unfold P. intros. inversion X. subst. Axiom cheat : forall P, P. apply cheat. apply cheat.
+  - intros. apply cheat.
+  - intros. subst. unfold P. intros. inversion X. subst. inversion X0. subst. apply T_Var. auto.
 Abort.
-      (*
-      inversion X0.
-      * subst.
-        simpl.
-        simpl in IHHt1.
-        apply IHHt1.
-        apply X.
-      * subst.
-        simpl.
-      *)
 
-(** *** Weakening of kinding *)
-Lemma weakening__has_kind : forall ctx ctx' T K,
-    (forall e, In e ctx -> In e ctx') ->
-    ctx |-* T : K ->
-    ctx' |-* T : K.
-Proof. Admitted.
-
-Lemma weakening__binding_well_formed : forall ctx ctx' b,
-    (forall e, In e ctx -> In e ctx') ->
-    ctx |-ok b ->
-    ctx' |-ok b.
-Proof. Admitted.
-
-Lemma CNR_Bindings__preserves_typing : forall bs ctx t_body T f_bs t_body',
-    (concat_rev_ctx (Lists.List.map binds bs) ++ ctx) |-+ t_body' : T ->
-    ctx |-+ (Let NonRec bs t_body) : T ->
-    CNR_Bindings bs f_bs ->
-    ctx |-+ (Lists.List.fold_right apply t_body' f_bs) : T.
-Proof.
-  intros.
-  generalize dependent t_body.
-  generalize dependent t_body'.
-  generalize dependent T.
-  generalize dependent ctx.
-  induction X.
-  - simpl. intros. 
-    inversion H0.
-    + subst.
-      assumption.
-    + subst.
-      assumption.
-  - intros.
-    inversion H0.
-    + subst.
-      inversion c.
-      subst.
-      simpl.
-      apply T_Apply with ty.
-      * apply T_LamAbs.
-        -- eapply IHX.
-            ++ unfold concat_rev_ctx in H.
-               simpl in H.
-               rewrite concat_app in H.
-               simpl in H.
-               rewrite <- app_assoc in H.
-               simpl in H.
-               apply H.
-            ++ apply T_Let.
-               ** apply weakening__has_kind with ctx.
-                  --- intros.
-                      destruct e; right; auto.
-                  --- auto. 
-               ** intros.
-                  apply weakening__binding_well_formed with ctx.
-                  --- intros. apply in_cons. apply H2.
-                  --- apply H5.
-                      apply in_cons. 
-                      apply H1.
-               ** simpl in H.
-                  unfold concat_rev_ctx in H.
-                  simpl in H.
-                  rewrite concat_app in H.
-                  simpl in H.
-                  rewrite <- app_assoc in H.
-                  simpl in H.
-                  apply H.
-        -- remember (H5 (TermBind Strict (VarDecl v ty) t_bound)).
-           clear Heqb.
-           assert (In (TermBind Strict (VarDecl v ty) t_bound) (TermBind Strict (VarDecl v ty) t_bound :: bs)). {
-             simpl. left. auto.
-           }
-           apply b in H1.
-           inversion H1. subst.
-           apply H8.
-      * remember (H5 (TermBind Strict (VarDecl v ty) t_bound)).
-        clear Heqb.
-        assert (In (TermBind Strict (VarDecl v ty) t_bound) (TermBind Strict (VarDecl v ty) t_bound :: bs)). {
-          simpl. left. auto.
-        }
-        apply b in H1.
-        inversion H1. subst.
-Abort.
